Foundation/Modal/Hilbert/WithRE_Normal.lean
@@ -6,63 +6,40 @@ namespace LO.Modal
 
 open LO.Modal.Entailment
 
-lemma Hilbert.equiv_WithRE_Normal
-  {HE : Hilbert.WithRE α} {HN : Hilbert.Normal α}
-  [RE HN] [Necessitation HE]
-  (provable_HE : ∀ φ ∈ HE.axiomInstances, HN ⊢! φ)
-  (provable_HN : ∀ φ ∈ HN.axiomInstances, HE ⊢! φ)
-  : HE ≊ HN := by
-  apply Entailment.Equiv.iff.mpr;
+lemma equiv_WithRE_Normal_of_provable_axiomInstances
+  {AxE AxN : Axiom ℕ}
+  [Necessitation (Hilbert.WithRE AxE)] [RE (Hilbert.Normal AxN)]
+  (hN : (Hilbert.Normal AxN) ⊢!* AxE.instances)
+  (hE : (Hilbert.WithRE AxE) ⊢!* AxN.instances)
+  : (Hilbert.WithRE AxE) ≊ (Hilbert.Normal AxN) := by
+  apply Logic.equiv_of_provable;
   intro φ;
-  suffices HE ⊢! φ ↔ HN ⊢! φ by
-    simpa [Entailment.theory, Set.mem_setOf_eq];
   constructor;
   . intro h;
-    induction h using Hilbert.WithRE.rec! with
-    | mdp ihφψ ihφ => apply ihφψ ⨀ ihφ;
+    induction h using Modal.Hilbert.WithRE.rec! with
+    | axm s h => apply hN; grind;
     | re h => apply re! h;
-    | @axm ψ s h =>
-      apply provable_HE;
-      use ψ;
-      constructor;
-      . assumption;
-      . use s;
+    | mdp ihφψ ihφ => exact ihφψ ⨀ ihφ
     | _ => simp;
   . intro h;
-    induction h using Hilbert.Normal.rec! with
-    | mdp ihφψ ihφ => apply ihφψ ⨀ ihφ;
-    | nec ihφ => apply Entailment.nec! ihφ;
-    | @axm ψ s h =>
-      apply provable_HN;
-      use ψ;
-      constructor;
-      . assumption;
-      . use s;
+    induction h using Modal.Hilbert.Normal.rec! with
+    | axm s h => apply hE; grind;
+    | nec h => exact nec! h;
+    | mdp ihφψ ihφ => exact ihφψ ⨀ ihφ;
     | _ => simp;
 
-lemma Hilbert.equiv_logic_WithRE_Normal
-  {HE : Hilbert.WithRE α} {HN : Hilbert.Normal α}
-  [RE HN] [Necessitation HE]
-  (provable_HE : ∀ φ ∈ HE.axiomInstances, HN ⊢! φ)
-  (provable_HN : ∀ φ ∈ HN.axiomInstances, HE ⊢! φ)
-  : HE.logic ≊ HN.logic := by
-  apply Entailment.Equiv.iff.mpr;
-  intro φ;
-  suffices HE ⊢! φ ↔ HN ⊢! φ by simpa [Modal.Logic.iff_provable, Entailment.theory, Set.mem_setOf_eq];
-  exact Entailment.Equiv.iff.mp (Hilbert.equiv_WithRE_Normal provable_HE provable_HN) φ;
+instance : Modal.EMCN ≊ Modal.K := by
+  apply equiv_WithRE_Normal_of_provable_axiomInstances;
+  . rintro φ (⟨_, (rfl | rfl | rfl), ⟨_, rfl⟩⟩) <;> simp;
+  . rintro φ (⟨_, rfl, ⟨_, rfl⟩⟩); simp;
 
-instance : 𝐄𝐌𝐂𝐍 ≊ Modal.K := by
-  apply Hilbert.equiv_logic_WithRE_Normal;
-  . rintro _ ⟨φ, (rfl | rfl | rfl), ⟨_, rfl⟩⟩ <;> simp;
-  . rintro _ ⟨φ, rfl, ⟨_, rfl⟩⟩; simp;
-
-instance : 𝐄𝐌𝐂𝐍𝐓 ≊ Modal.KT := by
-  apply Hilbert.equiv_logic_WithRE_Normal;
+instance : Modal.EMCNT ≊ Modal.KT := by
+  apply equiv_WithRE_Normal_of_provable_axiomInstances;
   . rintro _ ⟨φ, (rfl | rfl | rfl | rfl), ⟨_, rfl⟩⟩ <;> simp;
   . rintro _ ⟨φ, (rfl | rfl), ⟨_, rfl⟩⟩ <;> simp;
 
-instance : 𝐄𝐌𝐂𝐍𝐓𝟒 ≊ Modal.S4 := by
-  apply Hilbert.equiv_logic_WithRE_Normal;
+instance : Modal.EMCNT4 ≊ Modal.S4 := by
+  apply equiv_WithRE_Normal_of_provable_axiomInstances;
   . rintro _ ⟨φ, (rfl | rfl | rfl | rfl | rfl), ⟨_, rfl⟩⟩ <;> simp;
   . rintro _ ⟨φ, (rfl | rfl | rfl), ⟨_, rfl⟩⟩ <;> simp;
 
