Foundation/Modal/Kripke/Hilbert.lean
@@ -7,24 +7,12 @@ open Formula
 open Kripke
 open Formula.Kripke
 
-variable {H H₁ H₂ : Hilbert.Normal ℕ} {Γ : Set (Formula ℕ)} {φ : Formula ℕ}
-variable {F : Kripke.Frame} {C : Kripke.FrameClass}
+namespace Kripke
 
+variable {Ax : Axiom ℕ} {φ : Formula ℕ}
+variable {F : Frame} {C : FrameClass}
 
-lemma eq_hilbert_logic_frameClass_logic {H : Hilbert.Normal ℕ} {C : FrameClass} [sound : Sound H C] [complete : Complete H C] : H.logic = C.logic := by
-  ext φ;
-  constructor;
-  . intro h;
-    apply sound.sound;
-    simpa;
-  . intro h;
-    simpa using complete.complete h;
-
-
-namespace Hilbert.Kripke
-
-
-lemma soundness_of_validates_axioms (hV : C ⊧* H.axioms) : H ⊢! φ → C ⊧ φ := by
+lemma soundness_of_validates_axioms (hV : C ⊧* Ax) : Hilbert.Normal Ax ⊢! φ → C ⊧ φ := by
   intro hφ F hF;
   induction hφ using Hilbert.Normal.rec! with
   | @axm φ s h =>
@@ -38,12 +26,14 @@ lemma soundness_of_validates_axioms (hV : C ⊧* H.axioms) : H ⊢! φ → C ⊧
   | imply₂ => exact ValidOnFrame.imply₂;
   | ec => exact ValidOnFrame.elimContra;
 
-instance instSound_of_validates_axioms (hV : C ⊧* H.axioms) : Sound H C := ⟨fun {_} =>
+instance instSound_of_validates_axioms (hV : C ⊧* Ax) : Sound (Hilbert.Normal Ax) C := ⟨fun {_} =>
   soundness_of_validates_axioms hV
 ⟩
 
-lemma consistent_of_sound_frameclass (C : Kripke.FrameClass) (C_nonempty: C.Nonempty := by simp)
-  [sound : Sound H C] : Entailment.Consistent H := by
+lemma consistent_of_sound_frameclass
+  (C : Kripke.FrameClass) (C_nonempty: C.Nonempty := by simp)
+  [sound : Sound (Hilbert.Normal Ax) C]
+  : Entailment.Consistent (Hilbert.Normal Ax) := by
   apply Entailment.Consistent.of_unprovable (φ := ⊥);
   apply not_imp_not.mpr sound.sound;
   apply Semantics.set_models_iff.not.mpr;
@@ -54,19 +44,7 @@ lemma consistent_of_sound_frameclass (C : Kripke.FrameClass) (C_nonempty: C.None
   . assumption;
   . simp;
 
-instance [Sound H C] : Sound H.logic C := by
-  constructor;
-  intro φ hφ;
-  apply Sound.sound (𝓢 := H);
-  grind;
-
-instance [Complete H C] : Complete H.logic C := by
-  constructor;
-  intro φ hφ;
-  suffices H ⊢! φ by grind;
-  apply Complete.complete hφ;
-
-lemma soundness_of_frame_validates_axioms (hV : F ⊧* H.axioms) : H ⊢! φ → F ⊧ φ := by
+lemma soundness_of_frame_validates_axioms (hV : F ⊧* Ax) : (Hilbert.Normal Ax) ⊢! φ → F ⊧ φ := by
   intro hφ;
   induction hφ using Hilbert.Normal.rec! with
   | axm s h =>
@@ -79,35 +57,26 @@ lemma soundness_of_frame_validates_axioms (hV : F ⊧* H.axioms) : H ⊢! φ →
   | imply₂ => exact ValidOnFrame.imply₂;
   | ec => exact ValidOnFrame.elimContra;
 
-instance instSound_of_frame_validates_axioms (hV : F ⊧* H.axioms) : Sound H F := ⟨fun {_} =>
+instance instSound_of_frame_validates_axioms (hV : F ⊧* Ax) : Sound (Hilbert.Normal Ax) F := ⟨fun {_} =>
   soundness_of_frame_validates_axioms hV
 ⟩
 
-lemma consistent_of_sound_frames (F : Kripke.Frame) [sound : Sound H F] : Entailment.Consistent H := by
+lemma consistent_of_sound_frames (F : Kripke.Frame) [sound : Sound (Hilbert.Normal Ax) F] : Entailment.Consistent (Hilbert.Normal Ax) := by
   apply Entailment.Consistent.of_unprovable (φ := ⊥);
   apply not_imp_not.mpr sound.sound;
   exact Kripke.ValidOnFrame.bot_def;
 
-lemma weakerThan_of_subset_frameClass (C₁ C₂ : FrameClass) (hC : C₂ ⊆ C₁) [Sound H₁ C₁] [Complete H₂ C₂] : H₁ ⪯ H₂ := by
+lemma weakerThan_of_subset_frameClass
+  (C₁ C₂ : FrameClass) (hC : C₂ ⊆ C₁)
+  [Sound (Hilbert.Normal Ax₁) C₁] [Complete (Hilbert.Normal Ax₂) C₂]
+  : (Hilbert.Normal Ax₁) ⪯ (Hilbert.Normal Ax₂) := by
   apply Entailment.weakerThan_iff.mpr;
   intro φ hφ;
   apply Complete.complete (𝓜 := C₂);
   intro F hF;
-  apply Sound.sound (𝓢 := H₁) (𝓜 := C₁) hφ;
+  apply Sound.sound (𝓜 := C₁) hφ;
   apply hC hF;
 
-instance [Sound H F] : Sound H.logic F := by
-  constructor;
-  intro φ hφ;
-  apply Sound.sound (𝓢 := H);
-  grind;
-
-instance [Complete H F] : Complete H.logic F := by
-  constructor;
-  intro φ hφ;
-  suffices H ⊢! φ by grind;
-  apply Complete.complete hφ;
-
-end Hilbert.Kripke
+end Kripke
 
 end LO.Modal
