Foundation/Modal/Kripke/Logic/K5.lean
@@ -1,6 +1,5 @@
 import Foundation.Modal.Kripke.AxiomGeach
 import Foundation.Modal.Kripke.Hilbert
-import Foundation.Modal.Hilbert.Normal.Basic
 import Foundation.Modal.Kripke.Logic.K
 
 namespace LO.Modal
@@ -8,7 +7,7 @@ namespace LO.Modal
 open Entailment
 open Formula
 open Kripke
-open Hilbert.Kripke
+open Modal.Kripke
 
 namespace Kripke
 
@@ -23,29 +22,29 @@ namespace Hilbert
 
 namespace K5.Kripke
 
-instance : Sound Hilbert.K5 FrameClass.K5 := instSound_of_validates_axioms $ by
+instance : Sound Modal.K5 FrameClass.K5 := instSound_of_validates_axioms $ by
   apply FrameClass.validates_with_AxiomK_of_validates;
   constructor;
   simp only [Set.mem_singleton_iff, forall_eq];
   rintro F F_eucl;
   exact validate_AxiomFive_of_euclidean (eucl := F_eucl);
 
-instance : Entailment.Consistent Hilbert.K5 :=
+instance : Entailment.Consistent Modal.K5 :=
   consistent_of_sound_frameclass FrameClass.K5 $ by
     use whitepoint;
     apply Set.mem_setOf_eq.mpr;
     infer_instance;
 
-instance : Canonical Hilbert.K5 FrameClass.K5 := ⟨by
+instance : Canonical Modal.K5 FrameClass.K5 := ⟨by
   apply Set.mem_setOf_eq.mpr;
   infer_instance;
 ⟩
 
-instance : Complete Hilbert.K5 FrameClass.K5 := inferInstance
+instance : Complete Modal.K5 FrameClass.K5 := inferInstance
 
 end K5.Kripke
 
-instance : Hilbert.K ⪱ Hilbert.K5 := by
+instance : Modal.K ⪱ Modal.K5 := by
   constructor;
   . apply Hilbert.Normal.weakerThan_of_subset_axioms $ by simp;
   . apply Entailment.not_weakerThan_iff.mpr;
@@ -64,7 +63,6 @@ instance : Hilbert.K ⪱ Hilbert.K5 := by
 
 end Hilbert
 
-instance : Modal.K ⪱ Modal.K5 := inferInstance
 
 
 end LO.Modal
