Foundation/Modal/Kripke/Logic/KB5.lean
@@ -1,13 +1,12 @@
 import Foundation.Modal.Kripke.AxiomGeach
 import Foundation.Modal.Kripke.Hilbert
-import Foundation.Modal.Hilbert.Normal.Basic
 
 namespace LO.Modal
 
 open Entailment
 open Formula
 open Kripke
-open Hilbert.Kripke
+open Modal.Kripke
 
 namespace Kripke
 
@@ -16,27 +15,19 @@ protected abbrev FrameClass.KB5 : FrameClass := { F | F.IsKB5 }
 
 end Kripke
 
-
-namespace Logic.KB5.Kripke
-
-instance : Sound (Hilbert.KB5) Kripke.FrameClass.KB5 := instSound_of_validates_axioms $ by
+instance : Sound (Modal.KB5) Kripke.FrameClass.KB5 := instSound_of_validates_axioms $ by
   apply FrameClass.validates_with_AxiomK_of_validates;
   constructor;
-  simp only [Set.mem_singleton_iff, forall_eq];
-  rintro F ⟨_, _⟩ _ (rfl | rfl);
+  rintro _ (rfl | rfl) F ⟨_, _⟩;
   . exact validate_AxiomB_of_symmetric;
   . exact validate_AxiomFive_of_euclidean;
 
-instance : Entailment.Consistent (Hilbert.KB5) := consistent_of_sound_frameclass Kripke.FrameClass.KB5 $ by
+instance : Entailment.Consistent (Modal.KB5) := consistent_of_sound_frameclass Kripke.FrameClass.KB5 $ by
   use whitepoint;
   constructor;
 
+instance : Canonical (Modal.KB5) Kripke.FrameClass.KB5 := ⟨by constructor⟩
 
-instance : Canonical (Hilbert.KB5) Kripke.FrameClass.KB5 := ⟨by constructor⟩
-
-instance : Complete (Hilbert.KB5) Kripke.FrameClass.KB5 := inferInstance
-
-end Logic.KB5.Kripke
-
+instance : Complete (Modal.KB5) Kripke.FrameClass.KB5 := inferInstance
 
 end LO.Modal
