Foundation/Modal/Kripke/Logic/S4H.lean
@@ -9,7 +9,7 @@ namespace LO.Modal
 open Entailment
 open Formula
 open Kripke
-open Hilbert.Kripke
+open Modal.Kripke
 
 
 namespace Kripke
@@ -27,11 +27,9 @@ instance [F.IsFiniteS4H] : F.IsFiniteGrz where
 end Kripke
 
 
-namespace Hilbert
+namespace S4H
 
-namespace S4H.Kripke
-
-instance : Sound (Hilbert.S4H) FrameClass.S4H := instSound_of_validates_axioms $ by
+instance : Sound (Modal.S4H) FrameClass.S4H := instSound_of_validates_axioms $ by
   apply FrameClass.validates_with_AxiomK_of_validates;
   constructor;
   rintro _ (rfl | rfl | rfl) F ⟨_, _⟩;
@@ -39,19 +37,20 @@ instance : Sound (Hilbert.S4H) FrameClass.S4H := instSound_of_validates_axioms $
   . exact validate_AxiomFour_of_transitive;
   . exact validate_axiomH_of_isDetourFree;
 
-instance : Entailment.Consistent (Hilbert.S4H) := consistent_of_sound_frameclass FrameClass.S4H $ by
+instance : Entailment.Consistent (Modal.S4H) := consistent_of_sound_frameclass FrameClass.S4H $ by
   use whitepoint;
   constructor;
 
-instance : Canonical (Hilbert.S4H) FrameClass.S4H := ⟨by constructor⟩
+instance : Canonical (Modal.S4H) FrameClass.S4H := ⟨by constructor⟩
 
-instance : Complete (Hilbert.S4H) FrameClass.S4H := inferInstance
+instance : Complete (Modal.S4H) FrameClass.S4H := inferInstance
 
-instance : Complete Hilbert.S4H FrameClass.finite_S4H := by sorry
+instance : Complete Modal.S4H FrameClass.finite_S4H := by sorry
 
-end S4H.Kripke
+end S4H
 
-instance : Hilbert.Grz ⪱ Hilbert.S4H := by
+
+instance : Modal.Grz ⪱ Modal.S4H := by
   constructor;
   . apply weakerThan_of_subset_frameClass (FrameClass.finite_Grz) (FrameClass.finite_S4H)
     intro F hF;
@@ -77,8 +76,5 @@ instance : Hilbert.Grz ⪱ Hilbert.S4H := by
           simp [M];
           omega;
 
-end Hilbert
-
-instance : Modal.Grz ⪱ Modal.S4H := inferInstance
 
 end LO.Modal
