Foundation/Modal/PLoN/Hilbert.lean
@@ -10,24 +10,26 @@ open Formula.PLoN
 namespace PLoN.Hilbert
 
 open Formula
-variable {C : PLoN.FrameClass}
-variable {H : Hilbert.Normal ℕ} {Γ : Set (Formula ℕ)} {φ : Formula ℕ}
 
-lemma soundness_of_defined_by_AxiomInstances [defined : C.DefinedBy H.axiomInstances] : H ⊢! φ → C ⊧ φ := by
+variable {Ax : Axiom ℕ} {φ : Formula ℕ}
+variable {F : Frame} {C : FrameClass}
+
+lemma soundness_of_defined_by_AxiomInstances [defined : C.DefinedBy Ax.instances] : Hilbert.Normal Ax ⊢! φ → C ⊧ φ := by
   intro hφ F hF;
   induction hφ using Hilbert.Normal.rec! with
-  | axm s h =>
+  | @axm φ s h =>
     apply defined.defines F |>.mp hF;
-    aesop;
+    use φ;
+    tauto;
   | mdp ihpq ihp => exact ValidOnFrame.mdp ihpq ihp;
   | nec ih => exact ValidOnFrame.nec ih;
   | imply₁ => exact ValidOnFrame.imply₁;
   | imply₂ => exact ValidOnFrame.imply₂;
   | ec => exact ValidOnFrame.elimContra;
 
-instance [C.DefinedBy H.axiomInstances] : Sound H C := ⟨fun {_} => soundness_of_defined_by_AxiomInstances⟩
+instance [C.DefinedBy Ax.instances] : Sound (Hilbert.Normal Ax) C := ⟨fun {_} => soundness_of_defined_by_AxiomInstances⟩
 
-lemma consistent_of_FrameClass_aux [nonempty : C.IsNonempty] [sound : Sound H C] : H ⊬ ⊥ := by
+lemma consistent_of_FrameClass_aux [nonempty : C.IsNonempty] [sound : Sound (Hilbert.Normal Ax) C] : (Hilbert.Normal Ax) ⊬ ⊥ := by
   apply not_imp_not.mpr sound.sound;
   apply ValidOnFrameClass.not_of_exists_frame;
   obtain ⟨F, hF⟩ := nonempty;
@@ -36,7 +38,7 @@ lemma consistent_of_FrameClass_aux [nonempty : C.IsNonempty] [sound : Sound H C]
   . assumption;
   . simp;
 
-lemma consistent_of_FrameClass (C : PLoN.FrameClass) [C.IsNonempty] [Sound H C] : Entailment.Consistent H := by
+lemma consistent_of_FrameClass (C : PLoN.FrameClass) [C.IsNonempty] [Sound (Hilbert.Normal Ax) C] : Entailment.Consistent (Hilbert.Normal Ax) := by
   apply Entailment.Consistent.of_unprovable;
   exact consistent_of_FrameClass_aux (C := C);
 
